

## Machine Learning

### Logistic regression and SVM

- Given historical data as below, if current weights  $\mathbf{W}$  for logistic regression model (in which  $P(y=1|\mathbf{X})=\sigma(\mathbf{W}^T\mathbf{X})$ ,  $\mathbf{X}=[x_1, x_2]^T$  is  $[0, 0]^T$ , update  $\mathbf{W}$  one step according to the gradient ascend. The learning rate  $\eta=0.1$

y	x1	x2
1	2	1
0	1	2
0	3	3

$$\mathbf{w}^{\text{new}} = \mathbf{w}^{\text{old}} + \eta \sum_t \left\{ y_n - \sigma \left( \left( \mathbf{w}^{\text{old}} \right)^T \mathbf{x}_n \right) \right\} \mathbf{x}_n.$$

$$=[0 \ 0]^T + 0.1 * \{ (1 - \sigma([0 \ 0] * [2 \ 1]^T)) * [2 \ 1]^T + (0 - \sigma([0 \ 0] * [1 \ 2]^T)) * [1 \ 2]^T + (0 - \sigma([0 \ 0] * [3 \ 3]^T)) * [3 \ 3]^T \}$$

$$=[0 \ 0]^T + 0.1 * \{ (1 - \sigma(0)) * [2 \ 1]^T + (0 - \sigma(0)) * [1 \ 2]^T + (0 - \sigma(0)) * [3 \ 3]^T \}$$

$$=[0 \ 0]^T + 0.1 * \{ 0.5 * [2 \ 1]^T - 0.5 * [1 \ 2]^T - 0.5 * [3 \ 3]^T \}$$

$$=[-0.1, -0.2]^T$$

2. Given a dataset as below, what is the solution of SVM model, where  $y = \text{sign}(\mathbf{W}^T \mathbf{X} + b)$ ,  $\mathbf{X} = [x_1, x_2]^T$ . That is, solve the  $\mathbf{W}$  and  $b$ . (Hint, solve the dual problem)

y	x1	x2
1	2	1
-1	1	2
-1	3	3

Dual problem

$$\begin{aligned} \max_{\alpha} \quad & \mathcal{G}(\alpha) = -\frac{1}{2} \sum_{i=1}^N \sum_{j=1}^N \alpha_i \alpha_j y_i y_j \mathbf{x}_i^T \mathbf{x}_j + \sum_{i=1}^N \alpha_i, \\ \text{subject to} \quad & \sum_{i=1}^N \alpha_i y_i = 0, \\ & \alpha_i \geq 0, \quad i = 1, \dots, N. \end{aligned}$$

Max  $G(a_1, a_2, a_3)$

$$\begin{aligned} = & -0.5 \{ (a_1 * a_1 * 1 * 1 * [2 \ 1]^T [2 \ 1]^T) + (a_1 * a_2 * 1 * (-1) * [2 \ 1]^T [1 \ 2]^T) + (a_1 * a_3 * 1 * (-1) * [2 \ 1]^T [3 \ 3]^T) \\ & + (a_2 * a_1 * (-1) * 1 * [1 \ 2]^T [2 \ 1]^T) + (a_2 * a_2 * (-1) * (-1) * [1 \ 2]^T [1 \ 2]^T) + (a_2 * a_3 * (-1) * (-1) * [1 \ 2]^T [3 \ 3]^T) \\ & + (a_3 * a_1 * (-1) * 1 * [3 \ 3]^T [2 \ 1]^T) + (a_3 * a_2 * (-1) * (-1) * [3 \ 3]^T [1 \ 2]^T) + (a_3 * a_3 * (-1) * (-1) * [3 \ 3]^T [3 \ 3]^T) \} \\ & + a_1 + a_2 + a_3 \end{aligned}$$

Subject to  $a_1 * 1 + a_2 * (-1) + a_3 * (-1) = 0$ ,  $a_1 \geq 0$ ,  $a_2 \geq 0$ ,  $a_3 \geq 0$

Max  $G(a_1, a_2, a_3)$

$$\begin{aligned} = & -0.5 \{ 5 * a_1 * a_1 - 4 * a_1 * a_2 - 9 * a_1 * a_3 \\ & - 4 * a_2 * a_1 + 5 * a_2 * a_2 + 9 * a_2 * a_3 \\ & - 9 * a_3 * a_1 + 9 * a_3 * a_2 + 18 * a_3 * a_3 \} \\ & + a_1 + a_2 + a_3 \end{aligned}$$

Subject to  $a_1 = a_2 + a_3$ ,  $a_1 \geq 0$ ,  $a_2 \geq 0$ ,  $a_3 \geq 0$

Replacing  $a_1 = a_2 + a_3$  into  $G$

Max  $G(a_2, a_3)$

$$\begin{aligned} = & -0.5 \{ 5 * (a_2 + a_3) * (a_2 + a_3) - 4 * (a_2 + a_3) * a_2 - 9 * (a_2 + a_3) * a_3 \\ & - 4 * a_2 * (a_2 + a_3) + 5 * a_2 * a_2 + 9 * a_2 * a_3 \\ & - 9 * a_3 * (a_2 + a_3) + 9 * a_3 * a_2 + 18 * a_3 * a_3 \} \\ & + a_2 + a_3 + a_2 + a_3 \end{aligned}$$

Subject to  $a_2 \geq 0$ ,  $a_3 \geq 0$

That is

Max  $G(a_2, a_3) = -a_2^2 * a_2 - 2.5 * a_3 * a_3 - a_2^2 * a_3 + 2 * a_2 * a_3$  (this is one degree 2 polynomial)

Subject to  $a_2 \geq 0$ ,  $a_3 \geq 0$

$$dG/da_2 = 0 \Rightarrow -2 * a_2 - a_3 + 2 = 0 \quad dG/da_3 = 0 \Rightarrow -5 * a_3 - a_2 + 2 = 0$$

$$\Rightarrow a_2 = 8/9, a_3 = 2/9 \Rightarrow a_1 = a_2 + a_3 = 10/9$$

$$\Rightarrow \mathbf{W} = a_1 * (1) * [2 \ 1]^T + a_2 * (-1) * [1 \ 2]^T + a_3 * (-1) * [3 \ 3]^T = [2/3 \ -4/3]^T$$

$a_1 > 0$ , so  $\mathbf{X} = [2 \ 1]^T$  is the support vector, for this  $\mathbf{X}$ , we have  $y(\mathbf{W}^T \mathbf{X} + b) = 1$  or  $1([2/3 \ -4/3]^T [2 \ 1]^T + b) = 1$

$$\Rightarrow b = 1$$